code/arch/x64/interop/Quad32_xor_win.fsti
@@ -35,6 +35,8 @@ let bufs_disjoint (ls:list s8) : Type0 = normalize (locs_disjoint_rec ls)
 unfold
 let buf_disjoint_from (b:s8) (ls:list s8) : Type0 = normalize (loc_locs_disjoint_rec b ls)
 
+unfold let disjoint_or_eq (#a:Type0) (b1:B.buffer a) (b2:B.buffer a) =
+  M.(loc_disjoint (loc_buffer b1) (loc_buffer b2)) \/ b1 == b2 
 
 let buffer_to_quad32 (b:s8 { B.length b % 16 == 0 /\ B.length b > 0 }) (h:HS.mem) : GTot quad32 =
   let b128 = BV.mk_buffer_view b Views.view128 in
@@ -45,7 +47,7 @@ let buffer_to_quad32 (b:s8 { B.length b % 16 == 0 /\ B.length b > 0 }) (h:HS.mem
   assert (BV.length b128 > 0);
   BV.sel h b128 0
 
-let pre_cond (h:HS.mem) (src1:s8) (src2:s8) (dst:s8) = live h src1 /\ live h src2 /\ live h dst /\ list_disjoint_or_eq [src1;src2;dst] /\     B.length src1 == 16 /\ B.length src2 == 16 /\ B.length dst == 16
+let pre_cond (h:HS.mem) (src1:s8) (src2:s8) (dst:s8) = live h src1 /\ live h src2 /\ live h dst /\ disjoint_or_eq src1 src2 /\ disjoint_or_eq src1 dst /\ disjoint_or_eq src2 dst /\     B.length src1 == 16 /\ B.length src2 == 16 /\ B.length dst == 16
 
 let post_cond (h:HS.mem) (h':HS.mem) (src1:s8) (src2:s8) (dst:s8) =
 B.length src1 == 16 /\ B.length src2 == 16 /\ B.length dst == 16 /\
